erc721/Model.v
@@ -1,0 +1,103 @@
+(*
+  This file is part of the verified smart contract project of SECBIT Labs.
+
+  Copyright 2018 SECBIT Labs
+
+  This program is free software: you can redistribute it and/or
+  modify it under the terms of the GNU Lesser General Public License
+  as published by the Free Software Foundation, either version 3 of
+  the License, or (at your option) any later version.
+
+  This program is distributed in the hope that it will be useful,
+  but WITHOUT ANY WARRANTY; without even the implied warranty of
+  MERCHANTABILITY or FITNESS FOR A PARTICULAR PURPOSE.  See the GNU
+  Lesser General Public License for more details.
+
+  You should have received a copy of the GNU Lesser General Public License
+  along with this program.  If not, see <https://www.gnu.org/licenses/>.
+*)
+
+Require Import
+        Integers
+        Lists.List
+        String
+        ZArith.
+Require Export
+        AbsModel
+        LibEx
+        Maps
+        Types.
+
+Record State : Type :=
+  mk_st {
+      st_tokenOwner: v2a;
+      st_tokenApprovals: v2a;
+      st_ownedTokensCount: a2v;
+      st_operatorApprovals: aa2b;
+    }.
+
+Record ReceiverState : Type :=
+  mk_rev_st {
+    }.
+
+Inductive Event : Type :=
+| ev_Transfer (this: address) (from: address) (to: address) (token_id: uint256)
+| ev_Approval (this: address) (owner: address) (approved: address) (token_id: uint256)
+| ev_ApprovalForAll (this: address) (owner: address) (operator: address) (approved: bool)
+| ev_constructor (sender: address)
+| ev_return {A: Type} (ret: A)
+| ev_revert (this: address)
+.
+
+Definition EventList := TEventList Event.
+
+Definition Env := TEnv ReceiverState.
+
+Definition Contract := TContract State.
+
+Inductive Mcall : Type :=
+| mc_constructor
+| mc_balanceOf (owner: address)
+| mc_ownerOf (token_id: uint256)
+| mc_safeTransferFrom (from: address) (to: address) (token_id: uint256) (data: option bytes)
+| mc_transferFrom (from: address) (to: address) (token_id: uint256)
+| mc_approve (approved: address) (token_id: uint256)
+| mc_setApprovalForAll (operator: address) (approved: bool)
+| mc_getApproved (token_id: uint256)
+| mc_isApprovedForAll (owner: address) (opeartor: address)
+| mc_supportsInterface (if_id: bytes4)
+| mc_mint (to: address) (token_id: uint256)
+.
+
+Definition Message := TMessage Mcall.
+
+Axiom safeTransferFrom_token_id_in_range:
+  forall msg from to id data,
+    m_func msg = mc_safeTransferFrom from to id data ->
+    0 <= id <= MAX_UINT256.
+
+Axiom transferFrom_token_id_in_range:
+  forall msg from to id,
+    m_func msg = mc_transferFrom from to id ->
+    0 <= id <= MAX_UINT256.
+
+Axiom approve_token_id_in_range:
+  forall msg approved id,
+    m_func msg = mc_approve approved id ->
+    0 <= id <= MAX_UINT256.
+
+Axiom getApproved_token_id_in_range:
+  forall msg id,
+    m_func msg = mc_getApproved id ->
+    0 <= id <= MAX_UINT256.
+
+Axiom ownedTokensCount_in_range:
+  forall addr st,
+    0 <= A2V.get (st_ownedTokensCount st) addr <= MAX_UINT256.
+    
+
+Parameter ERC721_INTERFACE_ID : bytes4.
+Parameter ERC165_INTERFACE_ID : bytes4.
+
+Axiom if_neq:
+  ERC721_INTERFACE_ID <> ERC165_INTERFACE_ID.
