erc721/Prop.v
@@ -1,0 +1,188 @@
+(*
+  This file is part of the verified smart contract project of SECBIT Labs.
+
+  Copyright 2018 SECBIT Labs
+
+  This program is free software: you can redistribute it and/or
+  modify it under the terms of the GNU Lesser General Public License
+  as published by the Free Software Foundation, either version 3 of
+  the License, or (at your option) any later version.
+
+  This program is distributed in the hope that it will be useful,
+  but WITHOUT ANY WARRANTY; without even the implied warranty of
+  MERCHANTABILITY or FITNESS FOR A PARTICULAR PURPOSE.  See the GNU
+  Lesser General Public License for more details.
+
+  You should have received a copy of the GNU Lesser General Public License
+  along with this program.  If not, see <https://www.gnu.org/licenses/>.
+*)
+
+Require Import Arith.
+Require Import Lists.List.
+Require Import Nat.
+Require Import Omega.
+
+Require Import Maps.
+Require Import Model.
+Require Import Spec.
+
+Definition assert_genesis_event (e: Event) (E: EventList) : Prop :=
+  match E with
+    | nil => False
+    | cons e' E => e = e'
+  end.
+
+Lemma assert_genesis_event_app :
+  forall e E E',
+    assert_genesis_event e E
+    -> assert_genesis_event e (E ++ E').
+Proof.
+  intros.
+  destruct E.
+  + simpl in H.  inversion H.
+  + simpl in H. auto.
+Qed.
+
+Definition PropINV (env: Env) (S: State) (E: EventList) : Prop :=
+  (exists creator,
+      assert_genesis_event (ev_constructor creator) E) /\
+  (forall owner,
+      owner <> 0 ->
+      length (V2A.map_filter (st_tokenOwner S) (fun e => Nat.eqb (snd e) owner)) =
+      (st_ownedTokensCount S $ owner)%a2v).
+
+Lemma create_INV :
+  forall env0 env msg C E,
+    create env0 msg C E
+    -> env_step env0 env
+    -> PropINV env (w_st C) E.
+Proof.
+  intros env0 env msg C evts Hcreate Henv_step.
+  destruct Hcreate; subst; simpl in *; subst.
+  split.
+
+  - exists sender.
+    constructor; auto.
+
+  - destruct H3 as [HtokenOwner [HtokenApprovals [HownedTokensCount HoperatorApprovals]]].
+    intros.
+    rewrite HownedTokensCount; A2V.msimpl.
+    rewrite (V2A.filter_length_equal _ HtokenOwner).
+    auto.
+Qed.
+
+Lemma step_INV:
+  forall this env msg S E env' S' E',
+    step env (mk_contract this S) msg (mk_contract this S') E'
+    -> env_step env env'
+    -> PropINV env S E
+    -> PropINV env' S' (E ++ E').
+Proof.
+  intros this env msg st evts env' st' evts' Hstep _ HPinv.
+
+  unfold PropINV in *.
+  destruct HPinv as [[creator Hcreator] HPinv].
+  split.
+
+  - exists creator. apply assert_genesis_event_app; auto.
+
+  - clear creator Hcreator.
+    intros owner Howner_nonzero.
+
+    inversion Hstep;
+      unfold func_step in H1;
+      destruct H1 as [Haddr [Hinv [Hinv' [Hreq [Hevts Htrans]]]]];
+      unfold INV in Hinv, Hinv';
+      subst;
+      simpl in *;
+      subst;
+      (* Htrans in some cases are simply 'C' = C' *)
+      try destruct Htrans as [HtokenOwner [HtokenApprovals [HownedTokensCount HoperatorApprovals]]];
+      auto.
+Qed.
+
+Lemma step_contract_address_preserve:
+  forall env C msg C' E',
+    step env C msg C' E'
+    -> w_a C = w_a C'.
+Proof.
+  intros.
+  destruct C as [a S].
+  destruct C' as [a' S'].
+  induction H; unfold func_step in H1; intuition.
+Qed.
+
+Lemma steps_INV:
+  forall ml env env' C C' E E',
+    PropINV env (w_st C) E ->
+    steps env C ml env' C' E' ->
+    PropINV env' (w_st C') (E ++ E').
+Proof.
+  induction ml; simpl.
+
+  - intros env env' C C' E E' HPinv [Hcontract [Hevts' Henv]].
+    subst. rewrite app_nil_r; auto.
+
+  - intros env env' C C' E E' HPinv Hsteps.
+    destruct Hsteps as [env'' [C'' [E'' [E''' [Hstep [Hsteps [HE' Henv_step]]]]]]].
+    destruct C. destruct C''.
+    simpl in *.
+
+    generalize (step_contract_address_preserve _ _ _ _ _ Hstep);
+      simpl; intros HC_eq.
+
+    rewrite HC_eq in Hstep.
+    generalize (step_INV _ _ _ _ _ _ _ _ Hstep Henv_step HPinv);
+      intros HPinv''.
+    substH IHml with
+        (IHml env'' env' {| w_a := w_a0; w_st := w_st0 |} C' (E ++ E'') E'''
+              HPinv'' Hsteps).
+    simpl in IHml.
+    subst E'.
+    rewrite (app_assoc _ _ _).
+    auto.
+Qed.
+
+(* Prop #1: owned token count consistency *)
+Theorem Property_owned_token_count_consistency:
+  forall env0 msg0 env ml C E C' E',
+    create env0 msg0 C E
+    -> env_step env0 env
+    -> run env C ml C' E'
+    -> forall owner,
+        owner <> 0 ->
+        length (V2A.map_filter (st_tokenOwner (w_st C')) (fun e => Nat.eqb (snd e) owner)) =
+        (st_ownedTokensCount (w_st C') $ owner)%a2v.
+Proof.
+  intros env0 msg0 env ml C evts C' evts'
+         Hcreate Henv_step Hrun owner Howner_nonzero.
+  inversion Hrun; subst.
+  generalize (create_INV env0 env msg0 C evts Hcreate Henv_step);
+    intros HPinv.
+  generalize (steps_INV _ _ _ _ _ _ _ HPinv H);
+    intros HPinv'.
+
+  unfold PropINV in HPinv'.
+  destruct HPinv' as [_ HPinv'].
+  apply HPinv'; auto.
+Qed.
+
+(* Prop #2: every newly minted token is unique *)
+Theorem Property_unique_minted_token:
+  forall msg to token,
+    m_func msg = mc_mint to token ->
+    forall env C C' evts,
+      step env C msg C' evts ->
+      st_tokenOwner (w_st C) $ token = 0.
+Proof.
+  intros msg to token Hfunc env C C' evts Hstep.
+
+  inversion Hstep; subst;
+    try inversion Hfunc;
+    subst.
+
+  unfold func_step in H1.
+  destruct H1 as [Hst [_ [_ [Hreq _]]]].
+  unfold funcspec_mint in Hreq; simpl in Hreq.
+  intuition.
+Qed.
