libs/wip/A2B.v
@@ -1,22 +1,3 @@
-(*
-  This file is part of the verified smart contract project of SECBIT Labs.
-
-  Copyright 2018 SECBIT Labs
-
-  This program is free software: you can redistribute it and/or
-  modify it under the terms of the GNU Lesser General Public License
-  as published by the Free Software Foundation, either version 3 of
-  the License, or (at your option) any later version.
-
-  This program is distributed in the hope that it will be useful,
-  but WITHOUT ANY WARRANTY; without even the implied warranty of
-  MERCHANTABILITY or FITNESS FOR A PARTICULAR PURPOSE.  See the GNU
-  Lesser General Public License for more details.
-
-  You should have received a copy of the GNU Lesser General Public License
-  along with this program.  If not, see <https://www.gnu.org/licenses/>.
-*)
-
 Require Import Mapping.
 Require Import ElemTypes.
 Require Import Types.
@@ -30,10 +11,10 @@ Notation "m '$' k" :=
   (A2B.get m k)
     (at level 50, left associativity, only parsing) : a2b_scope.
 
-Notation "m '$=' m'" :=
-  (A2B.equal m m')
-    (at level 50, left associativity, only parsing) : a2b_scope.
-
 Notation "m '$' '{' k '<~' v '}'" :=
   (A2B.upd m k v)
     (at level 50, left associativity, only parsing) : a2b_scope.
+
+Notation "m '~' m'" :=
+  (A2B.equal m m')
+    (at level 70, no associativity, only parsing) : a2b_scope.
