libs/wip/AA2B.v
@@ -1,0 +1,45 @@
+Require Import ZArith.
+Require Import DecidableType.
+
+Require Import Mapping.
+Require Import ElemTypes.
+Require Import Types.
+
+Module AA_as_DT := DecidableTypeEx.PairDecidableType (Address_as_DT) (Address_as_DT).
+
+Module AA2B := Mapping (AA_as_DT) (BoolElem).
+Definition aa2b := AA2B.t.
+
+Notation "$0" := (AA2B.empty) (only parsing) : aa2b_scope.
+
+Notation "m '$' '[' k0 ',' k1 ']'" :=
+  (AA2B.get m (k0, k1))
+    (at level 50, left associativity, only parsing) : aa2b_scope.
+
+Notation "m '$' '{' k0 ',' k1 '<~' v '}'" :=
+  (AA2B.upd m (k0, k1) v)
+    (at level 50, left associativity, only parsing) : aa2b_scope.
+
+Notation "m '~' m'" :=
+  (AA2B.equal m m')
+    (at level 70, no associativity, only parsing) : aa2b_scope.
+
+Open Scope aa2b_scope.
+
+Section EqDec.
+  Lemma aa_eqdec:
+    forall (k k': address * address),
+      { (fun x y : nat * nat => fst x = fst y /\ snd x = snd y) k k' } +
+      { ~ (fun x y : nat * nat => fst x = fst y /\ snd x = snd y) k k' }.
+  Proof.
+    intros.
+    destruct k as [a0 a1].
+    destruct k' as [a0' a1'].
+    destruct (Nat.eq_dec a0 a0'); destruct (Nat.eq_dec a1 a1');
+      solve [ left; auto |
+              right;
+              intros Heq; inversion Heq;
+              apply n; auto
+            ].
+  Qed.
+End EqDec.
