libs/wip/AA2V.v
@@ -1,22 +1,3 @@
-(*
-  This file is part of the verified smart contract project of SECBIT Labs.
-
-  Copyright 2018 SECBIT Labs
-
-  This program is free software: you can redistribute it and/or
-  modify it under the terms of the GNU Lesser General Public License
-  as published by the Free Software Foundation, either version 3 of
-  the License, or (at your option) any later version.
-
-  This program is distributed in the hope that it will be useful,
-  but WITHOUT ANY WARRANTY; without even the implied warranty of
-  MERCHANTABILITY or FITNESS FOR A PARTICULAR PURPOSE.  See the GNU
-  Lesser General Public License for more details.
-
-  You should have received a copy of the GNU Lesser General Public License
-  along with this program.  If not, see <https://www.gnu.org/licenses/>.
-*)
-
 Require Import ZArith.
 Require Import DecidableType.
 
@@ -35,10 +16,6 @@ Notation "m '$' '[' k0 ',' k1 ']'" :=
   (AA2V.get m (k0, k1))
     (at level 50, left associativity, only parsing) : aa2v_scope.
 
-Notation "m '$=' m'" :=
-  (AA2V.equal m m')
-    (at level 50, left associativity, only parsing) : aa2v_scope.
-
 Notation "m '$' '{' k0 ',' k1 '<~' v '}'" :=
   (AA2V.upd m (k0, k1) v)
     (at level 50, left associativity, only parsing) : aa2v_scope.
@@ -50,6 +27,10 @@ Notation "m '$' '{' k0 ',' k1  '<+~' v '}'" :=
 Notation "m '$' '{' k0 ',' k1 '<-~' v '}'" :=
   (AA2V.upd_dec m (k0, k1) v)
     (at level 50, left associativity, only parsing) : aa2v_scope.
+
+Notation "m '~' m'" :=
+  (AA2V.equal m m')
+    (at level 70, no associativity, only parsing) : aa2v_scope.
 
 Open Scope aa2v_scope.
 
