libs/wip/V2A.v
@@ -1,0 +1,23 @@
+Require Import Mapping.
+Require Import ElemTypes.
+Require Import Types.
+Require Import LibEx.
+
+Module Import V2A := Mapping (UINT256_as_DT) (AddrElem).
+Definition v2a: Type := V2A.t.
+
+Notation "$0" := (V2A.empty) (only parsing) : v2a_scope.
+
+Notation "m '$' k" :=
+  (V2A.get m k)
+    (at level 50, left associativity, only parsing) : v2a_scope.
+
+Notation "m '$' '{' k '<~' v '}'" :=
+  (V2A.upd m k v)
+    (at level 50, left associativity, only parsing) : v2a_scope.
+
+Notation "m '~' m'" :=
+  (V2A.equal m m')
+    (at level 70, no associativity, only parsing) : v2a_scope.
+
+Open Scope v2a_scope.
