Makefile
@@ -2,6 +2,7 @@ include config.mk
 
 SUBDIRS := erc20 erc20_burnable erc20_pausable erc20_mintable erc20_lockable
 SUBDIRS += erc20_upgradable
+SUBDIRS += erc721
 
 all: $(SUBDIRS)
 	@for dir in $(SUBDIRS); do \
